LeanLoris/Scratch.lean
@@ -1,0 +1,23 @@
+open Nat
+
+def slowFib (id : Nat) : Nat → Nat
+  | 0   => 1
+  | 1   => 1
+  | n+2 => dbgTrace s!"fib {id}" fun _ => slowFib id n + slowFib id (n+1)
+
+-- def conc : Nat := 
+--   let t1 := Task.spawn fun _ => slowFib 1 32
+--   let t2 := Task.spawn fun _ => slowFib 2 32
+--   let t3 := Task.spawn fun _ => slowFib 3 33
+--   let t4 := Task.spawn fun _ => slowFib 4 34
+--   t1.get + t2.get + t3.get + t4.get
+
+-- #eval conc
+
+def conc2 : Nat :=
+  let arr := #[1, 3, 4, 5, 6]
+  let tsks := arr.map fun n => Task.spawn fun _ => slowFib n (30 + n)
+  let res := tsks.map fun t => t.get
+  res.foldl (fun acc n => acc + n) 0
+
+#eval conc2
